If we put cs_cont_equiv as a hypothesis to sync, transitivity doesn't hold. And if we try to make sync stronger by quantifying over any possible (k1,k1') pair, reflexivity doesn't hold, but probably it should, we'd have to prove that if we swap k1 by an equivalent k1', execution stays in sync, which seems to be an important property, but currently that doesn't hold when we return from Kcall and restore env/temp_env

ifc/ifc_def.v
@@ -195,39 +195,58 @@ Definition sync (ge : genv) (s1: corestate) (m1: mem) (s2: corestate) (m2: mem):
 *)
 
 Definition sync (ge : genv) (s1: corestate) (m1: mem) (s1': corestate) (m1': mem): Prop :=
+  cs_cont_equiv s1 s1' ->
   forall s2 m2 n, starN ge n s1 m1 s2 m2 ->
     exists s2' m2', starN ge n s1' m1' s2' m2' /\ cs_cont_equiv s2 s2'.
-
-Lemma sync_to_cs_cont_equiv: forall ge s1 m1 s1' m1',
-  sync ge s1 m1 s1' m1' -> cs_cont_equiv s1 s1'.
-Proof.
-  unfold sync. introv Sy. specialize (Sy s1 m1 O). simpl in Sy.
-  specialize (Sy eq_refl). destruct Sy as [x [y [Eq CE]]]. inversion Eq. subst x y.
-  assumption.
-Qed.
-
-Lemma sync_refl: forall (ge : genv) (s: corestate) (m: mem),
-  sync ge s m s m.
-Proof.
-  intros. unfold sync.
-  introv Star. pose proof cs_cont_equiv_refl. eauto.
-Qed.
-
-Lemma sync_sym: forall (ge : genv) (s1 s1': corestate) (m1 m1' : mem),
-  sync ge s1 m1 s1' m1' -> sync ge s1' m1' s1 m1.
-Abort. (* Doesn't hold, but we don't need it. *)
 
 Lemma sync_trans: forall ge s1 s2 s3 m1 m2 m3,
   sync ge s1 m1 s2 m2 -> sync ge s2 m2 s3 m3 -> sync ge s1 m1 s3 m3.
 Proof.
-  introv Sy12 Sy23. unfold sync.
-  intros s1' m1' n Star1.
+  introv Sy12 Sy23. unfold sync in *.
+  intros CE13 s1' m1' n Star1.
+  edestruct Sy12 as [s2' [m2' [Star2 CE12']]].
+  (* can't get (cs_cont_equiv s1 s2)  *)
+Abort. (*
+  
   specialize (Sy12 _ _ _ Star1).
-  destruct Sy12 as [s2' [m2' [Star2 CE12']]].
   specialize (Sy23 _ _ _ Star2).
   destruct Sy23 as [s3' [m3' [Star3 CE23']]].
   pose proof cs_cont_equiv_trans. eauto.
 Qed.
+*)
+
+Reset sync.
+
+Definition sync (ge : genv) (e1 : env) (te1 : temp_env) (m1 : mem)
+                            (e1': env) (te1': temp_env) (m1': mem): Prop
+:= forall k1 k1', cont_equiv k1 k1' ->
+   forall n e2  te2  k2  m2 , starN ge n (State e1  te1  k1 ) m1  (State e2  te2  k2 ) m2  ->
+     exists e2' te2' k2' m2', starN ge n (State e1' te1' k1') m1' (State e2' te2' k2') m2'
+                           /\ cont_equiv k2 k2'.
+
+(*
+Lemma sync_to_cs_cont_equiv: forall ge s1 m1 s1' m1',
+  sync ge s1 m1 s1' m1' -> cs_cont_equiv s1 s1'.
+Proof.
+Abort. doesn't hold any more
+  unfold sync. introv Sy. specialize (Sy s1 m1 O). simpl in Sy.
+  specialize (Sy eq_refl). destruct Sy as [x [y [Eq CE]]]. inversion Eq. subst x y.
+  assumption.
+Qed.
+*)
+
+Lemma sync_refl: forall (ge : genv) (e1 : env) (te1 : temp_env) (m1 : mem),
+  sync ge e1 te1 m1 e1 te1 m1.
+Proof.
+  intros. unfold sync.
+  introv CE Star. pose proof cont_equiv_refl.
+  (* Have to prove that if we swap k1 by an equivalent k1', execution stays in sync.
+     Doesn't hold when we return from Kcall and restore env/temp_env *)
+Abort.
+
+Lemma sync_sym: forall (ge : genv) (s1 s1': corestate) (m1 m1' : mem),
+  sync ge s1 m1 s1' m1' -> sync ge s1' m1' s1 m1.
+Abort. (* Doesn't hold, but we don't need it. *)
 
 Definition iguard {A : Type}
   (preP: A -> state_pred) (preN: A -> stack_clsf) (preA: A -> heap_clsf)
